wip: working on finite branching

fairness/lawyer/obligations/obligations_fin_branch.v
@@ -1,8 +1,9 @@
-From iris.algebra Require Import auth gmap gset excl excl_auth.
+From iris.algebra Require Import auth gmap gset excl excl_auth gmultiset.
 From iris.proofmode Require Import tactics.
 From trillium.fairness Require Import locales_helpers comp_utils trace_lookup fairness.
 From trillium.fairness.lawyer Require Import sub_action_em action_model.
-From trillium.fairness.lawyer.obligations Require Import obligations_model obligations_em obligations_am obls_fairness_preservation.
+From trillium.fairness.lawyer.obligations Require Import obligations_model obligations_em obligations_am obls_fairness_preservation obls_utils.
+From stdpp Require Import finite. 
 
 Section FiniteBranching.
   Context {DegO LevelO: ofe}.
@@ -22,9 +23,314 @@ Section FiniteBranching.
   Context (OP: ObligationsParams Degree Level Locale LIM_STEPS).
   Let OM := ObligationsModel OP.
 
-  Context `{Inhabited Locale}. 
+  Context `{Inhabited Locale}.
 
-  Theorem OM_fin_branch c δ
+  (* TODO: move / find implementation *)
+  Definition gset_prod `{Countable K, Countable T} (k: gset K) (t: gset T):
+    gset (K * T).
+    clear H3 H1 H0 H. 
+  Admitted.
+
+  Lemma gset_prod_spec `{Countable K, Countable T} (k: gset K) (t: gset T):
+    forall p, p ∈ gset_prod k t <-> p.1 ∈ k /\ p.2 ∈ t.
+  Proof using. Admitted.
+
+  (* TODO: move *)
+  Definition list_approx {A: Type} (P: A -> Prop) :=
+    { l: list A | forall a, P a -> a ∈ l }. 
+
+  Lemma burns_cp_next_states δ:
+    list_approx (fun δ' => exists τ π d, burns_cp OP δ τ δ' π d). 
+  Proof using.
+    set (new_cps := map (fun cp => ps_cps _ δ ∖ {[+ cp +]}) (elements $ ps_cps _ δ)).
+    exists (map (flip (update_cps OP) δ) new_cps). 
+    intros ? (?&?&? & STEP).
+    inversion STEP; subst; simpl in *. simpl.
+    apply elem_of_list_In. apply in_map_iff. eexists. simpl. split; [reflexivity|].
+    subst new_cps. apply in_map_iff. eexists. split; [reflexivity| ].
+    apply elem_of_list_In. apply gmultiset_elem_of_elements. done.
+  Qed.
+
+  Lemma exchanges_cp_next_states δ d':
+    list_approx (fun δ' => exists τ π d n, exchanges_cp OP δ τ δ' π d d' n). 
+  Proof using.
+    set (new_cps :=
+           '(π, d) ← elements $ ps_cps _ δ;
+           n ← seq 0 (ps_exc_bound _ δ + 1);
+           mret (ps_cps _ δ ∖ {[+ (π, d) +]} ⊎ n *: {[+ (π, d') +]})).
+    exists (map (flip (update_cps OP) δ) new_cps). 
+    intros ? (?&?&?&?& STEP).
+    inversion STEP; subst; simpl in *. simpl.
+    apply elem_of_list_In. apply in_map_iff. eexists. simpl. split; [reflexivity|].
+    subst new_cps. apply elem_of_list_In.
+    apply elem_of_list_bind. eexists (_, _). split.
+    2: { apply gmultiset_elem_of_elements. eauto. }
+    apply elem_of_list_bind. eexists. rewrite elem_of_list_ret. split; [reflexivity| ].
+    apply elem_of_seq. lia.
+  Qed.
+
+  Lemma creates_signal_next_states δ ℓ:
+    list_approx (fun δ' => exists τ, creates_signal OP δ τ δ' ℓ).
+  Proof using.
+    set (s := next_sig_id _ δ). 
+    set (new_sigs := <[ s := (ℓ, false) ]> (ps_sigs _ δ)).
+    set (add_obl := 
+           fun τ =>
+             let cur_loc_obls := default ∅ (ps_obls _ δ !! τ) in
+             <[ τ := cur_loc_obls ∪ {[ s ]} ]> (ps_obls _ δ)). 
+    set (new_obls := map add_obl (elements $ dom $ ps_obls _ δ)).
+    exists (map (flip (update_obls OP) (update_sigs OP new_sigs δ)) new_obls).
+    intros ? (?& STEP).
+    inversion STEP; subst; simpl in *. simpl.
+    apply elem_of_list_In. apply in_map_iff. eexists. split; [reflexivity|].
+    subst new_obls1. apply elem_of_list_In.
+    subst new_obls. apply elem_of_list_In, in_map_iff. eexists. split; [reflexivity|].
+    apply elem_of_list_In, elem_of_elements. done.
+  Qed.
+
+  Lemma sets_signal_next_states δ:
+    list_approx (fun δ' => exists τ s, sets_signal OP δ τ δ' s). 
+  Proof using.
+    set (set_sig τs' :=
+           let '(τ, s') := τs' in 
+           let new_sigs := (map_imap (fun s '(ℓ, b) => Some (ℓ, (if (decide (s' = s)) then true else b))) (ps_sigs _ δ)) in
+           let new_obls :=
+             (let cur_loc_obls := default ∅ (ps_obls _ δ !! τ) in
+              <[ τ := cur_loc_obls ∖ {[ s' ]} ]> (ps_obls _ δ)) in
+           update_obls OP new_obls $ update_sigs OP new_sigs δ
+           ). 
+    exists (map set_sig (elements $ gset_prod (dom $ ps_obls _ δ) (dom $ ps_sigs _ δ))).
+    intros ? (?&?& STEP). inversion STEP; subst; simpl in *. simpl.
+    apply elem_of_list_In. apply in_map_iff.
+    eexists (_, _). subst set_sig new_ps. split.
+    { f_equal. f_equal. subst new_sigs0.
+      apply map_eq. intros sid. rewrite map_lookup_imap. 
+      destruct (decide (sid = x0)) as [->|?].
+      { rewrite lookup_insert. rewrite SIG. simpl. rewrite decide_True; done. }
+      rewrite lookup_insert_ne; [| done]. 
+      destruct (ps_sigs OP δ !! sid) eqn:SID; rewrite SID; [| done].
+      simpl. destruct s. rewrite decide_False; done. }
+    apply elem_of_list_In, elem_of_elements.
+    apply gset_prod_spec. simpl. split; eauto.
+    by apply elem_of_dom.
+  Qed.
+
+  Lemma creates_ep_next_states δ d':
+    list_approx (fun δ' => exists τ s π d, creates_ep OP δ τ δ' s π d d'). 
+  Proof using.
+    set (add_ep s_cp :=
+           let '(s, (π, d)) := s_cp in
+           let new_cps := ps_cps _ δ ∖ {[+ (π, d) +]} in
+           let new_eps := ps_eps _ δ ∪ {[ (s, π, d') ]} in
+           update_eps _ new_eps $ update_cps _ new_cps δ).
+    exists (map add_ep (elements $ gset_prod (dom $ ps_sigs _ δ) (gmultiset_dom $ ps_cps _ δ))).
+    intros ? (?&?&?&?& STEP). inversion STEP; subst; simpl in *. simpl.
+    apply elem_of_list_In. apply in_map_iff.
+    eexists (_, (_, _)). split; [reflexivity| ].
+    apply elem_of_list_In, elem_of_elements.
+    apply gset_prod_spec. simpl. split; eauto.
+    by apply gmultiset_elem_of_dom.
+  Qed.
+
+  Lemma expects_ep_next_states δ:
+    list_approx (fun δ' => exists τ s π d, expects_ep OP δ τ δ' s π d).
+  Proof using.
+    set (add_cp (ep: @ExpectPermission Degree) := let '(_, π, d) := ep in ps_cps _ δ ⊎ {[+ (π, d) +]}).
+    exists (map (flip (update_cps OP) δ ∘ add_cp) (elements $ ps_eps _ δ)).
+    intros ? (?&?&?&?& STEP). inversion STEP; subst; simpl in *. simpl.
+    apply elem_of_list_In. apply in_map_iff. eexists ((_, _), _). split; [reflexivity| ].
+    apply elem_of_list_In, elem_of_elements. eauto.
+  Qed. 
+
+  Lemma forks_locale_next_states δ τ':
+    list_approx (fun δ' => exists τ obls', forks_locale _ δ τ δ' τ' obls'). 
+  Proof using.
+    clear H1 H0 H. 
+    exists (τπ0 ← map_to_list (ps_phases _ δ);
+           let '(τ, π0) := τπ0 in
+           let obls0 := default ∅ (ps_obls _ δ !! τ) in
+           obls' ← elements $ powerset obls0;           
+           let new_obls := <[ τ' := obls']> $ <[ τ := obls0 ∖ obls' ]> $ ps_obls _ δ in
+           let new_phases := <[ τ' := fork_right π0 ]> $ <[ τ := fork_left π0 ]> $ ps_phases _ δ in
+           mret (update_phases _ new_phases $ update_obls _ new_obls δ)).
+    intros ? (?&?& STEP). inversion STEP; subst; simpl in *. simpl. 
+    apply elem_of_list_bind. eexists (_, _).
+    rewrite elem_of_list_bind. setoid_rewrite elem_of_list_ret.
+    split.
+    { eexists. split; [reflexivity| ].
+      apply elem_of_elements. apply powerset_spec. set_solver. }
+    by apply elem_of_map_to_list. 
+  Qed.
+    
+  Lemma ex_and_comm' {T: Type} (A: Prop) (B: T -> Prop):
+    (exists t, B t /\ A) <-> (exists t, B t) /\ A.
+  Proof. 
+    split.
+    - intros (?&?&?); eauto.
+    - intros ((?&?)&?); eauto.
+  Qed.
+
+  Section FinParams.
+    Context (FINdeg: Finite Degree) (FINlvl: Finite Level).
+
+    Lemma loc_step_approx δ:
+      list_approx (fun δ' => exists τ, loc_step OP δ τ δ'). 
+    Proof using FINlvl FINdeg.
+      exists (
+          proj1_sig (burns_cp_next_states δ) ++
+            flat_map (fun d' => proj1_sig (exchanges_cp_next_states δ d')) (@enum _ _ FINdeg) ++
+            flat_map (fun ℓ => proj1_sig (creates_signal_next_states δ ℓ)) (@enum _ _ FINlvl) ++
+            proj1_sig (sets_signal_next_states δ) ++
+            flat_map (fun d' => proj1_sig (creates_ep_next_states δ d')) (@enum _ _ FINdeg) ++
+            proj1_sig (expects_ep_next_states δ)
+        ).
+      intros ? (?& STEP).
+      rewrite !elem_of_app. 
+      destruct STEP as [T|[T|[T|[T|[T|T]]]]]. 
+      - destruct T as (?&?&T). left.
+        destruct (burns_cp_next_states δ); eauto. 
+      - destruct T as (?&?&?&?&T). do 1 right. left.
+        apply elem_of_list_In, in_flat_map. setoid_rewrite <- elem_of_list_In.      
+        eexists. split.
+        { eapply elem_of_enum. Unshelve. eauto. }
+        destruct exchanges_cp_next_states; eauto.
+        eapply e; eauto. 
+      - destruct T as (?&T). do 2 right. left.
+        apply elem_of_list_In, in_flat_map. setoid_rewrite <- elem_of_list_In.      
+        eexists. split.
+        { eapply elem_of_enum. Unshelve. eauto. }
+        destruct creates_signal_next_states; eauto.
+      - destruct T as (?&T). do 3 right. left.
+        destruct sets_signal_next_states; eauto.
+      - destruct T as (?&?&?&?&T). do 4 right. left.
+        apply elem_of_list_In, in_flat_map. setoid_rewrite <- elem_of_list_In.      
+        eexists. split.
+        { eapply elem_of_enum. Unshelve. eauto. }
+        destruct creates_ep_next_states; eauto.
+        eapply e; eauto. 
+      - destruct T as (?&?&?&T). do 5 right.
+        destruct expects_ep_next_states; eauto.
+        eapply e; eauto. 
+    Qed.
+
+    Fixpoint list_approx_repeat {A : Type} (R: A -> A → Prop)
+      (APX: forall a, list_approx (R a))      
+      (n: nat)
+      (a: A)
+      :=
+      match n with
+      | 0 => [a]
+      | S n =>
+          let la := APX a in
+          flat_map (list_approx_repeat R APX n) (proj1_sig la)
+      end.
+
+    Lemma list_approx_repeat_spec {A} (R: A -> A -> Prop) APX n a:
+      forall b, relations.nsteps R n a b -> b ∈ list_approx_repeat R APX n a.
+    Proof using.
+      clear H1 H0 H. 
+      revert a. induction n.
+      { simpl. intros ??. rewrite nsteps_0. set_solver. }
+      intros ??. rewrite -rel_compose_nsteps_next'.       
+      intros (? & STEP & STEPS). 
+      apply IHn in STEPS. simpl.
+      apply elem_of_list_In. apply in_flat_map. eexists. split.
+      2: eapply elem_of_list_In; eauto.
+      destruct APX. simpl in *. apply elem_of_list_In. eauto.
+    Qed.
+
+    (* TODO: move *)
+    Instance nsteps_impl {A: Type}:
+      Proper ((eq ==> eq ==> impl) ==> eq ==> (eq ==> eq ==> impl)) (@relations.nsteps A).
+    Proof using.
+      red. intros ?????????????. subst. red in H4.
+      generalize dependent y2. induction y0.
+      { intros ?. by rewrite !nsteps_0. }
+      intros ?. rewrite -!rel_compose_nsteps_next.
+      intros (?&STEPS&STEP). apply IHy0 in STEPS.
+      eexists. split; eauto. eapply H4; eauto.
+    Qed. 
+
+    Lemma progress_step_approx δ:
+      list_approx (fun δ' => exists τ, progress_step OP δ τ δ'). 
+    Proof using FINlvl FINdeg.
+      clear H1 H0 H. 
+      red.
+      exists (flat_map (fun i => list_approx_repeat (fun δ1 δ2 => exists τ, loc_step _ δ1 τ δ2)
+                           loc_step_approx i δ) (seq 0 (LIM_STEPS + 2))).
+      intros δ' [τ STEP]. apply elem_of_list_In, in_flat_map.
+      setoid_rewrite <- elem_of_list_In.
+      red in STEP. destruct STEP as (n & LE & REL). exists (n + 1). split. 
+      { apply elem_of_seq. lia. }
+      eapply list_approx_repeat_spec.
+      destruct REL as (? & STEPS & STEP).
+      rewrite Nat.add_1_r. apply rel_compose_nsteps_next.
+      eexists. split.
+      2: { destruct STEP as (?&?&?). eexists.
+           red. left. eauto. }
+      eapply nsteps_impl; eauto.
+      red. intros ???????. subst. eauto.
+    Qed.
+
+    Lemma om_trans_approx δ (L: gset Locale):
+      list_approx (fun δ' => dom (ps_obls _ δ') ⊆ L /\ exists τ, om_trans OP δ τ δ'). 
+    Proof using FINlvl FINdeg.
+      clear H1 H0 H.
+      set (approx1 := proj1_sig $ progress_step_approx δ).
+      set (approx2 :=
+             τ' ← elements $ L;
+             δ' ← approx1;
+             proj1_sig (forks_locale_next_states δ' τ')).              
+      exists (approx1 ++ approx2).
+      intros δ' [LOCS [τ STEP]].
+      red in STEP. destruct STEP as (δ_ & PSTEP & FSTEP).
+      rewrite elem_of_app. inversion FSTEP; subst. 
+      2: { left. subst approx1. destruct progress_step_approx. eauto. }
+      right. subst approx2. apply elem_of_list_bind.
+      setoid_rewrite elem_of_list_bind.
+      destruct H as (τ' & ? & FORK). 
+      eexists. split; [eexists; split| ].
+      - destruct forks_locale_next_states. eauto.
+      - subst approx1. destruct progress_step_approx. eauto.
+      - apply elem_of_elements. inversion FORK. subst.
+        apply LOCS. subst ps'. destruct δ_. simpl in *.
+        subst new_obls0. rewrite dom_insert. set_solver.
+    Qed.
+      
+  End FinParams.
+
+  Theorem OM_fin_branch_impl c δ
+    (tp': list (language.expr Λ))
+    (σ': language.state Λ)
+    (oζ: olocale Λ):
+    exists nexts: list (ProgressState OP * (Action * option Locale)),
+      forall '(δ', ℓ),
+        obls_ves_wrapper OP c oζ (tp', σ') δ ℓ δ' ∧
+        om_live_tids OP id locale_enabled (tp', σ') δ' ->
+        (δ', ℓ) ∈ nexts.
+  Proof using.
+    assert (FINdeg: Finite Degree) by admit.
+    assert (FINlvl: Finite Level) by admit.
+    destruct (om_trans_approx _ _ δ (locales_of_cfg (tp', σ'))) as [nexts NEXTS].
+    exists (flat_map (fun τ => map (fun δ' => (δ', (obls_act, Some τ))) nexts) (elements $ locales_of_cfg c)).
+    intros [δ' [? oτ]] [STEP TIDS]. apply elem_of_list_In, in_flat_map.
+    setoid_rewrite <- elem_of_list_In.
+    simpl in STEP. destruct oτ as [τ| ]; [| tauto].
+    exists τ. simpl in STEP. destruct STEP as [STEP ->].
+    red in STEP. destruct STEP as (? & -> & TH_OWN). 
+    split.
+    { apply elem_of_elements.
+      admit. }
+    apply elem_of_list_In, in_map_iff. eexists. split; eauto.
+    apply elem_of_list_In. apply NEXTS. split.
+    2: { simpl in H4. eauto. }
+    red in TIDS.
+    by rewrite TH_OWN.
+  Qed. 
+
+    
+
+  Theorem OM_fin_branch_impl c δ
     (tp': list (language.expr Λ))
     (σ': language.state Λ)
     (oζ: olocale Λ):
@@ -33,7 +339,10 @@ Section FiniteBranching.
       obls_ves_wrapper OP c oζ (tp', σ') δ ℓ δ' ∧
       om_live_tids OP id locale_enabled (tp', σ') δ'} nat.
   Proof using.
-
+    unshelve eapply finitary.finite_smaller_card_nat.
+    { admit. }
+    
+    
   Admitted.     
 
 End FiniteBranching.
